Phi_Semantics/PhiSem_Mem_C_AI.thy
@@ -26,10 +26,10 @@ proc calloc_aN:
 
   semantic_local_value($n) \<open>\<a>\<i>\<n>\<t>\<close>
   semantic_assert \<open>Zero TY \<noteq> None\<close>
-  apply_rule FIC.aggregate_mem.allocate_rule[where TY=\<open>\<a>\<r>\<r>\<a>\<y>[nat (V_aint.dest (\<phi>arg.dest \<a>\<r>\<g>1))] TY\<close>
-                                               and v=\<open>sem_mk_array (replicate (nat (V_aint.dest (\<phi>arg.dest \<a>\<r>\<g>1))) (the (Zero TY)))\<close>]
+  apply_rule FIC.aggregate_mem.allocate_rule[where TY=\<open>\<a>\<r>\<r>\<a>\<y>[nat (sem_dest_aint (\<phi>arg.dest \<a>\<r>\<g>1))] TY\<close>
+                                               and v=\<open>sem_mk_array (replicate (nat (sem_dest_aint (\<phi>arg.dest \<a>\<r>\<g>1))) (the (Zero TY)))\<close>]
 
-  semantic_assumption \<open>type_storable_in_mem (\<a>\<r>\<r>\<a>\<y>[nat (V_aint.dest (\<phi>arg.dest \<a>\<r>\<g>1))] TY)\<close>
+  semantic_assumption \<open>type_storable_in_mem (\<a>\<r>\<r>\<a>\<y>[nat (sem_dest_aint (\<phi>arg.dest \<a>\<r>\<g>1))] TY)\<close>
 
   \<open>replicate n z \<Ztypecolon> MAKE _ (\<m>\<e>\<m>-\<b>\<l>\<k>[blk] (MAKE _ (\<m>\<e>\<m>-\<c>\<o>\<e>\<r>\<c>\<e> (Array n T))))\<close>
   \<open>replicate n z \<Ztypecolon> MAKE _ (\<m>\<e>\<m>[memaddr blk 0] (Array n T))\<close>
@@ -61,10 +61,10 @@ proc calloc_aN2:
 
   apply_rule FIC.aggregate_mem.allocate_rule
             [where TY=\<open>\<a>\<r>\<r>\<a>\<y>[n] \<a>\<r>\<r>\<a>\<y>[m] TY\<close>
-               and v=\<open>sem_mk_array (replicate (nat (V_aint.dest (\<phi>arg.dest \<a>\<r>\<g>1)))
-                                   (sem_mk_array (replicate (nat (V_aint.dest (\<phi>arg.dest \<a>\<r>\<g>2))) (the (Zero TY)))))\<close>]
+               and v=\<open>sem_mk_array (replicate (nat (sem_dest_aint (\<phi>arg.dest \<a>\<r>\<g>1)))
+                                   (sem_mk_array (replicate (nat (sem_dest_aint (\<phi>arg.dest \<a>\<r>\<g>2))) (the (Zero TY)))))\<close>]
 
-  semantic_assumption \<open>type_storable_in_mem (\<a>\<r>\<r>\<a>\<y>[nat (V_aint.dest (\<phi>arg.dest \<a>\<r>\<g>1))] \<a>\<r>\<r>\<a>\<y>[nat (V_aint.dest (\<phi>arg.dest \<a>\<r>\<g>2))] TY)\<close>
+  semantic_assumption \<open>type_storable_in_mem (\<a>\<r>\<r>\<a>\<y>[nat (sem_dest_aint (\<phi>arg.dest \<a>\<r>\<g>1))] \<a>\<r>\<r>\<a>\<y>[nat (sem_dest_aint (\<phi>arg.dest \<a>\<r>\<g>2))] TY)\<close>
 
   \<open>replicate n (replicate m z) \<Ztypecolon> MAKE _ (\<m>\<e>\<m>-\<b>\<l>\<k>[blk] (MAKE _ (\<m>\<e>\<m>-\<c>\<o>\<e>\<r>\<c>\<e> (Array n (Array m T)))))\<close>
   \<open>replicate n (replicate m z) \<Ztypecolon> MAKE _ (\<m>\<e>\<m>[memaddr blk 0] (Array n (Array m T)))\<close>
